clean Earley

CFG.thy
@@ -14,54 +14,54 @@ datatype 'a cfg =
   CFG (\<NN> : "'a list") (\<TT> : "'a list") (\<RR> : "'a rules") (\<SS> : "'a")
 
 definition disjunct_symbols :: "'a cfg \<Rightarrow> bool" where
-  "disjunct_symbols cfg \<equiv> set (\<NN> cfg) \<inter> set (\<TT> cfg) = {}"
+  "disjunct_symbols \<G> \<equiv> set (\<NN> \<G>) \<inter> set (\<TT> \<G>) = {}"
 
 definition valid_startsymbol :: "'a cfg \<Rightarrow> bool" where
-  "valid_startsymbol cfg \<equiv> \<SS> cfg \<in> set (\<NN> cfg)"
+  "valid_startsymbol \<G> \<equiv> \<SS> \<G> \<in> set (\<NN> \<G>)"
 
 definition valid_rules :: "'a cfg \<Rightarrow> bool" where
-  "valid_rules cfg \<equiv> \<forall>(N, \<alpha>) \<in> set (\<RR> cfg). N \<in> set (\<NN> cfg) \<and> (\<forall>s \<in> set \<alpha>. s \<in> set (\<NN> cfg) \<union> set (\<TT> cfg))"
+  "valid_rules \<G> \<equiv> \<forall>(N, \<alpha>) \<in> set (\<RR> \<G>). N \<in> set (\<NN> \<G>) \<and> (\<forall>s \<in> set \<alpha>. s \<in> set (\<NN> \<G>) \<union> set (\<TT> \<G>))"
 
 definition distinct_rules :: "'a cfg \<Rightarrow> bool" where
-  "distinct_rules cfg \<equiv> distinct (\<RR> cfg)"
+  "distinct_rules \<G> \<equiv> distinct (\<RR> \<G>)"
 
-definition wf_cfg :: "'a cfg \<Rightarrow> bool" where
-  "wf_cfg cfg \<equiv> disjunct_symbols cfg \<and> valid_startsymbol cfg \<and> valid_rules cfg \<and> distinct_rules cfg"
+definition wf_\<G> :: "'a cfg \<Rightarrow> bool" where
+  "wf_\<G> \<G> \<equiv> disjunct_symbols \<G> \<and> valid_startsymbol \<G> \<and> valid_rules \<G> \<and> distinct_rules \<G>"
 
-lemmas wf_cfg_defs = wf_cfg_def valid_rules_def valid_startsymbol_def disjunct_symbols_def distinct_rules_def
+lemmas wf_\<G>_defs = wf_\<G>_def valid_rules_def valid_startsymbol_def disjunct_symbols_def distinct_rules_def
 
 definition is_terminal :: "'a cfg \<Rightarrow> 'a \<Rightarrow> bool" where
-  "is_terminal cfg s \<equiv> s \<in> set (\<TT> cfg)"
+  "is_terminal \<G> x \<equiv> x \<in> set (\<TT> \<G>)"
 
 definition is_nonterminal :: "'a cfg \<Rightarrow> 'a \<Rightarrow> bool" where
-  "is_nonterminal cfg s \<equiv> s \<in> set (\<NN> cfg)"
+  "is_nonterminal \<G> x \<equiv> x \<in> set (\<NN> \<G>)"
 
 definition is_symbol :: "'a cfg \<Rightarrow> 'a \<Rightarrow> bool" where
-  "is_symbol cfg s \<equiv> is_terminal cfg s \<or> is_nonterminal cfg s"
+  "is_symbol \<G> x \<equiv> is_terminal \<G> x \<or> is_nonterminal \<G> x"
 
 definition wf_sentence :: "'a cfg \<Rightarrow> 'a sentence \<Rightarrow> bool" where
-  "wf_sentence cfg s \<equiv> \<forall>x \<in> set s. is_symbol cfg x"
+  "wf_sentence \<G> \<omega> \<equiv> \<forall>x \<in> set \<omega>. is_symbol \<G> x"
 
 lemma is_nonterminal_startsymbol:
-  "wf_cfg cfg \<Longrightarrow> is_nonterminal cfg (\<SS> cfg)"
-  by (simp add: is_nonterminal_def wf_cfg_defs)
+  "wf_\<G> \<G> \<Longrightarrow> is_nonterminal \<G> (\<SS> \<G>)"
+  by (simp add: is_nonterminal_def wf_\<G>_defs)
 
 definition is_word :: "'a cfg \<Rightarrow> 'a sentence \<Rightarrow> bool" where
-  "is_word cfg s = (\<forall>x \<in> set s. is_terminal cfg x)"
+  "is_word \<G> \<omega> \<equiv> \<forall>x \<in> set \<omega>. is_terminal \<G> x"
 
 definition derives1 :: "'a cfg \<Rightarrow> 'a sentence \<Rightarrow> 'a sentence \<Rightarrow> bool" where
-  "derives1 cfg u v \<equiv> \<exists> x y N \<alpha>. 
+  "derives1 \<G> u v \<equiv> \<exists> x y N \<alpha>. 
     u = x @ [N] @ y \<and>
     v = x @ \<alpha> @ y \<and>
-    (N, \<alpha>) \<in> set (\<RR> cfg)"  
+    (N, \<alpha>) \<in> set (\<RR> \<G>)"  
 
 definition derivations1 :: "'a cfg \<Rightarrow> ('a sentence \<times> 'a sentence) set" where
-  "derivations1 cfg \<equiv> { (u,v) | u v. derives1 cfg u v }"
+  "derivations1 \<G> \<equiv> { (u,v) | u v. derives1 \<G> u v }"
 
 definition derivations :: "'a cfg \<Rightarrow> ('a sentence \<times> 'a sentence) set" where 
-  "derivations cfg \<equiv> (derivations1 cfg)^*"
+  "derivations \<G> \<equiv> (derivations1 \<G>)^*"
 
 definition derives :: "'a cfg \<Rightarrow> 'a sentence \<Rightarrow> 'a sentence \<Rightarrow> bool" where
-  "derives cfg u v \<equiv> ((u, v) \<in> derivations cfg)"
+  "derives \<G> u v \<equiv> ((u, v) \<in> derivations \<G>)"
 
 end
