Derivations.thy
@@ -7,66 +7,66 @@ section \<open>Adjusted content from AFP/LocalLexing\<close>
 
 type_synonym 'a derivation = "(nat \<times> 'a rule) list"
 
-lemma [simp]: "is_word cfg []" by (auto simp add: is_word_def)
+lemma [simp]: "is_word \<G> []" by (auto simp add: is_word_def)
 
 lemma derives1_implies_derives[simp]:
-  "derives1 cfg a b \<Longrightarrow> derives cfg a b"
+  "derives1 \<G> a b \<Longrightarrow> derives \<G> a b"
   by (auto simp add: derives_def derivations_def derivations1_def)
 
 lemma derives_trans:
-  "derives cfg a b \<Longrightarrow> derives cfg b c \<Longrightarrow> derives cfg a c"
+  "derives \<G> a b \<Longrightarrow> derives \<G> b c \<Longrightarrow> derives \<G> a c"
   by (auto simp add: derives_def derivations_def)
 
 lemma derives1_eq_derivations1:
-  "derives1 cfg x y = ((x, y) \<in> derivations1 cfg)"
+  "derives1 \<G> x y = ((x, y) \<in> derivations1 \<G>)"
   by (simp add: derivations1_def)
 
 lemma derives_induct[consumes 1, case_names Base Step]:
-  assumes derives: "derives cfg a b"
+  assumes derives: "derives \<G> a b"
   assumes Pa: "P a"
-  assumes induct: "\<And>y z. derives cfg a y \<Longrightarrow> derives1 cfg y z \<Longrightarrow> P y \<Longrightarrow> P z"
+  assumes induct: "\<And>y z. derives \<G> a y \<Longrightarrow> derives1 \<G> y z \<Longrightarrow> P y \<Longrightarrow> P z"
   shows "P b"
 proof -
-  note rtrancl_lemma = rtrancl_induct[where a = a and b = b and r = "derivations1 cfg" and P=P]
+  note rtrancl_lemma = rtrancl_induct[where a = a and b = b and r = "derivations1 \<G>" and P=P]
   from derives Pa induct rtrancl_lemma show "P b"
     by (metis derives_def derivations_def derives1_eq_derivations1)
 qed
 
 definition Derives1 :: "'a cfg \<Rightarrow> 'a sentence \<Rightarrow> nat \<Rightarrow> 'a rule \<Rightarrow> 'a sentence \<Rightarrow> bool" where
-  "Derives1 cfg u i r v \<equiv> \<exists> x y N \<alpha>. 
+  "Derives1 \<G> u i r v \<equiv> \<exists> x y N \<alpha>. 
     u = x @ [N] @ y \<and>
     v = x @ \<alpha> @ y \<and>
-    (N, \<alpha>) \<in> set (\<RR> cfg) \<and> r = (N, \<alpha>) \<and> i = length x"  
+    (N, \<alpha>) \<in> set (\<RR> \<G>) \<and> r = (N, \<alpha>) \<and> i = length x"  
 
 lemma Derives1_split:
-  "Derives1 cfg u i r v \<Longrightarrow> \<exists> x y. u = x @ [fst r] @ y \<and> v = x @ (snd r) @ y \<and> length x = i"
+  "Derives1 \<G> u i r v \<Longrightarrow> \<exists> x y. u = x @ [fst r] @ y \<and> v = x @ (snd r) @ y \<and> length x = i"
   by (metis Derives1_def fst_conv snd_conv)
 
-lemma Derives1_implies_derives1: "Derives1 cfg u i r v \<Longrightarrow> derives1 cfg u v"
+lemma Derives1_implies_derives1: "Derives1 \<G> u i r v \<Longrightarrow> derives1 \<G> u v"
   by (auto simp add: Derives1_def derives1_def)
 
-lemma derives1_implies_Derives1: "derives1 cfg u v \<Longrightarrow> \<exists> i r. Derives1 cfg u i r v"
+lemma derives1_implies_Derives1: "derives1 \<G> u v \<Longrightarrow> \<exists> i r. Derives1 \<G> u i r v"
   by (auto simp add: Derives1_def derives1_def)
 
 fun Derivation :: "'a cfg \<Rightarrow> 'a sentence \<Rightarrow> 'a derivation \<Rightarrow> 'a sentence \<Rightarrow> bool" where
   "Derivation _ a [] b = (a = b)"
-| "Derivation cfg a (d#D) b = (\<exists> x. Derives1 cfg a (fst d) (snd d) x \<and> Derivation cfg x D b)"
+| "Derivation \<G> a (d#D) b = (\<exists> x. Derives1 \<G> a (fst d) (snd d) x \<and> Derivation \<G> x D b)"
 
-lemma Derivation_implies_derives: "Derivation cfg a D b \<Longrightarrow> derives cfg a b"
+lemma Derivation_implies_derives: "Derivation \<G> a D b \<Longrightarrow> derives \<G> a b"
 proof (induct D arbitrary: a b)
   case Nil thus ?case 
     by (simp add: derives_def derivations_def)
 next
   case (Cons d D)
   note ihyps = this
-  from ihyps have "\<exists> x. Derives1 cfg a (fst d) (snd d) x \<and> Derivation cfg x D b" by auto
-  then obtain x where "Derives1 cfg a (fst d) (snd d) x" and xb: "Derivation cfg x D b" by blast
-  with Derives1_implies_derives1 have d1: "derives cfg a x" by fastforce
-  from ihyps xb have d2:"derives cfg x b" by simp
-  show "derives cfg a b" by (rule derives_trans[OF d1 d2])
+  from ihyps have "\<exists> x. Derives1 \<G> a (fst d) (snd d) x \<and> Derivation \<G> x D b" by auto
+  then obtain x where "Derives1 \<G> a (fst d) (snd d) x" and xb: "Derivation \<G> x D b" by blast
+  with Derives1_implies_derives1 have d1: "derives \<G> a x" by fastforce
+  from ihyps xb have d2:"derives \<G> x b" by simp
+  show "derives \<G> a b" by (rule derives_trans[OF d1 d2])
 qed 
 
-lemma Derivation_Derives1: "Derivation cfg a S y \<Longrightarrow> Derives1 cfg y i r z \<Longrightarrow> Derivation cfg a (S@[(i,r)]) z"
+lemma Derivation_Derives1: "Derivation \<G> a S y \<Longrightarrow> Derives1 \<G> y i r z \<Longrightarrow> Derivation \<G> a (S@[(i,r)]) z"
 proof (induct S arbitrary: a y z i r)
   case Nil thus ?case by simp
 next
@@ -74,47 +74,47 @@ next
     by (metis Derivation.simps(2) append_Cons) 
 qed
 
-lemma derives_implies_Derivation: "derives cfg a b \<Longrightarrow> \<exists> D. Derivation cfg a D b"
+lemma derives_implies_Derivation: "derives \<G> a b \<Longrightarrow> \<exists> D. Derivation \<G> a D b"
 proof (induct rule: derives_induct)
   case Base
   show ?case by (rule exI[where x="[]"], simp)
 next
   case (Step y z)
   note ihyps = this
-  from ihyps obtain D where ay: "Derivation cfg a D y" by blast
-  from ihyps derives1_implies_Derives1 obtain i r where yz: "Derives1 cfg y i r z" by blast
+  from ihyps obtain D where ay: "Derivation \<G> a D y" by blast
+  from ihyps derives1_implies_Derives1 obtain i r where yz: "Derives1 \<G> y i r z" by blast
   from Derivation_Derives1[OF ay yz] show ?case by auto
 qed
 
-lemma rule_nonterminal_type[simp]: "wf_cfg cfg \<Longrightarrow> (N, \<alpha>) \<in> set (\<RR> cfg) \<Longrightarrow> is_nonterminal cfg N"
-  by (auto simp add: is_nonterminal_def wf_cfg_defs)
+lemma rule_nonterminal_type[simp]: "wf_\<G> \<G> \<Longrightarrow> (N, \<alpha>) \<in> set (\<RR> \<G>) \<Longrightarrow> is_nonterminal \<G> N"
+  by (auto simp add: is_nonterminal_def wf_\<G>_defs)
 
-lemma [elim]: "Derives1 cfg a i r b \<Longrightarrow> r \<in> set (\<RR> cfg)"
+lemma [elim]: "Derives1 \<G> a i r b \<Longrightarrow> r \<in> set (\<RR> \<G>)"
   using Derives1_def by metis
 
-lemma is_terminal_nonterminal: "wf_cfg cfg \<Longrightarrow> is_terminal cfg x \<Longrightarrow> is_nonterminal cfg x \<Longrightarrow> False"
-  by (auto simp: wf_cfg_defs disjoint_iff is_nonterminal_def is_terminal_def)
+lemma is_terminal_nonterminal: "wf_\<G> \<G> \<Longrightarrow> is_terminal \<G> x \<Longrightarrow> is_nonterminal \<G> x \<Longrightarrow> False"
+  by (auto simp: wf_\<G>_defs disjoint_iff is_nonterminal_def is_terminal_def)
 
-lemma is_word_is_terminal: "i < length u \<Longrightarrow> is_word cfg u \<Longrightarrow> is_terminal cfg (u ! i)"
+lemma is_word_is_terminal: "i < length u \<Longrightarrow> is_word \<G> u \<Longrightarrow> is_terminal \<G> (u ! i)"
   using is_word_def by force
 
-lemma Derivation_append: "Derivation cfg a (D@E) c = (\<exists> b. Derivation cfg a D b \<and> Derivation cfg b E c)"
+lemma Derivation_append: "Derivation \<G> a (D@E) c = (\<exists> b. Derivation \<G> a D b \<and> Derivation \<G> b E c)"
   by (induct D arbitrary: a c E) auto
 
 lemma Derivation_implies_append: 
-  "Derivation cfg a D b \<Longrightarrow> Derivation cfg b E c \<Longrightarrow> Derivation cfg a (D@E) c"
+  "Derivation \<G> a D b \<Longrightarrow> Derivation \<G> b E c \<Longrightarrow> Derivation \<G> a (D@E) c"
   using Derivation_append by blast
 
 
 section \<open>Additional derivation lemmas\<close>
 
 lemma Derives1_prepend:
-  assumes "Derives1 cfg u i r v"
-  shows "Derives1 cfg (w@u) (i + length w) r (w@v)"
+  assumes "Derives1 \<G> u i r v"
+  shows "Derives1 \<G> (w@u) (i + length w) r (w@v)"
 proof -
   obtain x y N \<alpha> where *:
     "u = x @ [N] @ y" "v = x @ \<alpha> @ y"
-    "(N, \<alpha>) \<in> set (\<RR> cfg)" "r = (N, \<alpha>)" "i = length x"
+    "(N, \<alpha>) \<in> set (\<RR> \<G>)" "r = (N, \<alpha>)" "i = length x"
     using assms Derives1_def by (smt (verit))
   hence "w@u = w @ x @ [N] @ y" "w@v = w @ x @ \<alpha> @ y"
     by auto
@@ -126,16 +126,16 @@ proof -
 qed
 
 lemma Derivation_prepend:
-  "Derivation cfg b D b' \<Longrightarrow> Derivation cfg (a@b) (map (\<lambda>(i, r). (i + length a, r)) D) (a@b')"
+  "Derivation \<G> b D b' \<Longrightarrow> Derivation \<G> (a@b) (map (\<lambda>(i, r). (i + length a, r)) D) (a@b')"
   using Derives1_prepend by (induction D arbitrary: b b') (auto, fast)
 
 lemma Derives1_append:
-  assumes "Derives1 cfg u i r v"
-  shows "Derives1 cfg (u@w) i r (v@w)"
+  assumes "Derives1 \<G> u i r v"
+  shows "Derives1 \<G> (u@w) i r (v@w)"
 proof -
   obtain x y N \<alpha> where *: 
     "u = x @ [N] @ y" "v = x @ \<alpha> @ y"
-    "(N, \<alpha>) \<in> set (\<RR> cfg)" "r = (N, \<alpha>)" "i = length x"
+    "(N, \<alpha>) \<in> set (\<RR> \<G>)" "r = (N, \<alpha>)" "i = length x"
     using assms Derives1_def by (smt (verit))
   hence "u@w = x @ [N] @ y @ w" "v@w = x @ \<alpha> @ y @ w"
     by auto
@@ -147,31 +147,31 @@ proof -
 qed
 
 lemma Derivation_append':
-  "Derivation cfg a D a' \<Longrightarrow> Derivation cfg (a@b) D (a'@b)"
+  "Derivation \<G> a D a' \<Longrightarrow> Derivation \<G> (a@b) D (a'@b)"
   using Derives1_append by (induction D arbitrary: a a') (auto, fast)
 
 lemma Derivation_append_rewrite:
-  assumes "Derivation cfg a D (b @ c @ d) " "Derivation cfg c E c'"
-  shows "\<exists>F. Derivation cfg a F (b @ c' @ d)"
+  assumes "Derivation \<G> a D (b @ c @ d) " "Derivation \<G> c E c'"
+  shows "\<exists>F. Derivation \<G> a F (b @ c' @ d)"
   using assms Derivation_append' Derivation_prepend Derivation_implies_append by fast
 
 lemma derives1_if_valid_rule:
-  "(N, \<alpha>) \<in> set (\<RR> cfg) \<Longrightarrow> derives1 cfg [N] \<alpha>"
+  "(N, \<alpha>) \<in> set (\<RR> \<G>) \<Longrightarrow> derives1 \<G> [N] \<alpha>"
   unfolding derives1_def
   apply (rule_tac exI[where x="[]"])
   apply (rule_tac exI[where x="[]"])
   by simp
 
 lemma derives_if_valid_rule:
-  "(N, \<alpha>) \<in> set (\<RR> cfg) \<Longrightarrow> derives cfg [N] \<alpha>"
+  "(N, \<alpha>) \<in> set (\<RR> \<G>) \<Longrightarrow> derives \<G> [N] \<alpha>"
   using derives1_if_valid_rule by fastforce
 
 lemma Derivation_from_empty:
-  "Derivation cfg [] D a \<Longrightarrow> a = []"
+  "Derivation \<G> [] D a \<Longrightarrow> a = []"
   by (cases D) (auto simp: Derives1_def)
 
 lemma Derivation_concat_split:
-  "Derivation cfg (a@b) D c \<Longrightarrow> \<exists>E F a' b'. Derivation cfg a E a' \<and> Derivation cfg b F b' \<and>
+  "Derivation \<G> (a@b) D c \<Longrightarrow> \<exists>E F a' b'. Derivation \<G> a E a' \<and> Derivation \<G> b F b' \<and>
      c = a' @ b' \<and> length E \<le> length D \<and> length F \<le> length D"
 proof (induction D arbitrary: a b)
   case Nil
@@ -179,10 +179,10 @@ proof (induction D arbitrary: a b)
     by (metis Derivation.simps(1) order_refl)
 next
   case (Cons d D)
-  then obtain ab where *: "Derives1 cfg (a@b) (fst d) (snd d) ab" "Derivation cfg ab D c"
+  then obtain ab where *: "Derives1 \<G> (a@b) (fst d) (snd d) ab" "Derivation \<G> ab D c"
     by auto
   then obtain x y N \<alpha> where #:
-    "a@b = x @ [N] @ y" "ab = x @ \<alpha> @ y" "(N,\<alpha>) \<in> set (\<RR> cfg)" "snd d = (N,\<alpha>)" "fst d = length x"
+    "a@b = x @ [N] @ y" "ab = x @ \<alpha> @ y" "(N,\<alpha>) \<in> set (\<RR> \<G>)" "snd d = (N,\<alpha>)" "fst d = length x"
     using * unfolding Derives1_def by blast
   show ?case
   proof (cases "length a \<le> length x")
@@ -193,17 +193,17 @@ next
       "ab = take (length a) x @ drop (length a) x @ \<alpha> @ y"
       using #(1,2) True by (metis append_eq_append_conv_if)+
     then obtain E F a' b' where IH:
-      "Derivation cfg (take (length a) x) E a'"
-      "Derivation cfg (drop (length a) x @ \<alpha> @ y) F b'"
+      "Derivation \<G> (take (length a) x) E a'"
+      "Derivation \<G> (drop (length a) x @ \<alpha> @ y) F b'"
       "c = a' @ b'"
       "length E \<le> length D"
       "length F \<le> length D"
       using Cons *(2) by blast
-    have "Derives1 cfg b (fst d - length a) (snd d) (drop (length a) x @ \<alpha> @ y)"
+    have "Derives1 \<G> b (fst d - length a) (snd d) (drop (length a) x @ \<alpha> @ y)"
       unfolding Derives1_def using *(1) #(3-5) ab_def(2) by (metis length_drop)
-    hence "Derivation cfg b ((fst d - length a, snd d) # F) b'"
+    hence "Derivation \<G> b ((fst d - length a, snd d) # F) b'"
       using IH(2) by force
-    moreover have "Derivation cfg a E a'"
+    moreover have "Derivation \<G> a E a'"
       using IH(1) ab_def(1) by fastforce
     ultimately show ?thesis
       using IH(3-5) by fastforce
@@ -217,21 +217,39 @@ next
     have "ab = x @ \<alpha> @ take (length a - length x - 1) y @ drop (length a - length x - 1) y"
       using #(2) by force
     then obtain E F a' b' where IH:
-      "Derivation cfg (x @ \<alpha> @ take (length a - length x - 1) y) E a'"
-      "Derivation cfg (drop (length a - length x - 1) y) F b'"
+      "Derivation \<G> (x @ \<alpha> @ take (length a - length x - 1) y) E a'"
+      "Derivation \<G> (drop (length a - length x - 1) y) F b'"
       "c = a' @ b'"
       "length E \<le> length D"
       "length F \<le> length D"
       using Cons.IH[of "x @ \<alpha> @ take (length a - length x - 1) y" "drop (length a - length x - 1) y"] *(2) by auto
-    have "Derives1 cfg a (fst d) (snd d) (x @ \<alpha> @ take (length a - length x - 1) y)"
+    have "Derives1 \<G> a (fst d) (snd d) (x @ \<alpha> @ take (length a - length x - 1) y)"
       unfolding Derives1_def using #(3-5) a_def by blast
-    hence "Derivation cfg a ((fst d, snd d) # E) a'"
+    hence "Derivation \<G> a ((fst d, snd d) # E) a'"
       using IH(1) by fastforce
-    moreover have "Derivation cfg b F b'"
+    moreover have "Derivation \<G> b F b'"
       using b_def IH(2) by blast
     ultimately show ?thesis
       using IH(3-5) by fastforce
   qed
+qed
+
+lemma Derivation_\<SS>1:
+  assumes "Derivation \<G> [\<SS> \<G>] D \<omega>" "is_word \<G> \<omega>" "wf_\<G> \<G>"
+  shows "\<exists>\<alpha> E. Derivation \<G> \<alpha> E \<omega> \<and> (\<SS> \<G>,\<alpha>) \<in> set (\<RR> \<G>)"
+proof (cases D)
+  case Nil
+  thus ?thesis
+    using assms is_nonterminal_startsymbol is_terminal_nonterminal by (metis Derivation.simps(1) is_word_def list.set_intros(1))
+next
+  case (Cons d D)
+  then obtain \<alpha> where "Derives1 \<G> [\<SS> \<G>] (fst d) (snd d) \<alpha>" "Derivation \<G> \<alpha> D \<omega>"
+    using assms by auto
+  hence "(\<SS> \<G>, \<alpha>) \<in> set (\<RR> \<G>)"
+    unfolding Derives1_def
+    by (metis List.append.right_neutral List.list.discI append_eq_Cons_conv append_is_Nil_conv nth_Cons_0 self_append_conv2)
+  thus ?thesis
+    using \<open>Derivation \<G> \<alpha> D \<omega>\<close> by auto
 qed
 
 end
