Earley.thy
@@ -1,7 +1,6 @@
 theory Earley
   imports
     Derivations
-    Limit
 begin
 
 section \<open>Slices\<close>
@@ -23,7 +22,7 @@ lemma slice_append_aux:
 lemma slice_concat:
   "a \<le> b \<Longrightarrow> b \<le> c \<Longrightarrow> slice a b xs @ slice b c xs = slice a c xs"
   apply (induction a b xs arbitrary: c rule: slice.induct)
-  apply (auto simp: slice_append_aux)
+     apply (auto simp: slice_append_aux)
   using Suc_le_D by fastforce
 
 lemma slice_concat_Ex:
@@ -74,62 +73,58 @@ lemma slice_singleton:
 
 section \<open>Earley recognizer\<close>
 
-subsection \<open>Earley Items\<close>
+subsection \<open>Earley items\<close>
 
 definition rule_head :: "'a rule \<Rightarrow> 'a" where
-  "rule_head = fst"
+  "rule_head \<equiv> fst"
 
 definition rule_body :: "'a rule \<Rightarrow> 'a list" where
-  "rule_body = snd"
+  "rule_body \<equiv> snd"
 
 datatype 'a item = 
-  Item 
-    (item_rule: "'a rule") 
-    (item_dot : nat) 
-    (item_origin : nat)
-    (item_end : nat)
+  Item (item_rule: "'a rule") (item_dot : nat) (item_origin : nat) (item_end : nat)
 
 definition item_rule_head :: "'a item \<Rightarrow> 'a" where
-  "item_rule_head x = rule_head (item_rule x)"
+  "item_rule_head x \<equiv> rule_head (item_rule x)"
 
 definition item_rule_body :: "'a item \<Rightarrow> 'a sentence" where
-  "item_rule_body x = rule_body (item_rule x)"
+  "item_rule_body x \<equiv> rule_body (item_rule x)"
 
 definition item_\<alpha> :: "'a item \<Rightarrow> 'a sentence" where
-  "item_\<alpha> x = take (item_dot x) (item_rule_body x)"
+  "item_\<alpha> x \<equiv> take (item_dot x) (item_rule_body x)"
 
 definition item_\<beta> :: "'a item \<Rightarrow> 'a sentence" where 
-  "item_\<beta> x = drop (item_dot x) (item_rule_body x)"
+  "item_\<beta> x \<equiv> drop (item_dot x) (item_rule_body x)"
 
 definition is_complete :: "'a item \<Rightarrow> bool" where
-  "is_complete x = (item_dot x \<ge> length (item_rule_body x))"
+  "is_complete x \<equiv> item_dot x \<ge> length (item_rule_body x)"
 
 definition next_symbol :: "'a item \<Rightarrow> 'a option" where
-  "next_symbol x = (if is_complete x then None else Some (item_rule_body x ! item_dot x))"
+  "next_symbol x \<equiv> if is_complete x then None else Some (item_rule_body x ! item_dot x)"
 
 lemmas item_defs = item_rule_head_def item_rule_body_def item_\<alpha>_def item_\<beta>_def rule_head_def rule_body_def
 
 definition is_finished :: "'a cfg \<Rightarrow> 'a sentence \<Rightarrow> 'a item \<Rightarrow> bool" where
-  "is_finished cfg inp x \<equiv>
-    item_rule_head x = \<SS> cfg \<and>
+  "is_finished \<G> \<omega> x \<equiv>
+    item_rule_head x = \<SS> \<G> \<and>
     item_origin x = 0 \<and>
-    item_end x = length inp \<and> 
+    item_end x = length \<omega> \<and> 
     is_complete x"
 
-definition earley_recognized :: "'a item set \<Rightarrow> 'a cfg \<Rightarrow> 'a sentence \<Rightarrow> bool" where
-  "earley_recognized I cfg inp = (\<exists>x \<in> I. is_finished cfg inp x)"
+definition recognizing :: "'a item set \<Rightarrow> 'a cfg \<Rightarrow> 'a sentence \<Rightarrow> bool" where
+  "recognizing I \<G> \<omega> \<equiv> \<exists>x \<in> I. is_finished \<G> \<omega> x"
 
 inductive_set Earley :: "'a cfg \<Rightarrow> 'a sentence \<Rightarrow> 'a item set"
   for \<G> :: "'a cfg" and \<omega> :: "'a sentence" where
-  Init: "r \<in> set (\<RR> \<G>) \<Longrightarrow> fst r = \<SS> \<G>
+    Init: "r \<in> set (\<RR> \<G>) \<Longrightarrow> fst r = \<SS> \<G>
     \<Longrightarrow> Item r 0 0 0 \<in> Earley \<G> \<omega>"
-| Scan: "x = Item r b i j \<Longrightarrow> x \<in> Earley \<G> \<omega> \<Longrightarrow>
+  | Scan: "x = Item r b i j \<Longrightarrow> x \<in> Earley \<G> \<omega> \<Longrightarrow>
     \<omega>!j = a \<Longrightarrow> j < length \<omega> \<Longrightarrow> next_symbol x = Some a \<Longrightarrow>
       Item r (b + 1) i (j + 1) \<in> Earley \<G> \<omega>"
-| Predict: "x = Item r b i j \<Longrightarrow> x \<in> Earley \<G> \<omega> \<Longrightarrow>
+  | Predict: "x = Item r b i j \<Longrightarrow> x \<in> Earley \<G> \<omega> \<Longrightarrow>
     r' \<in> set (\<RR> \<G>) \<Longrightarrow> next_symbol x = Some (rule_head r') \<Longrightarrow>
       Item r' 0 j j \<in> Earley \<G> \<omega>"
-| Complete: "x = Item r\<^sub>x b\<^sub>x i j \<Longrightarrow> x \<in> Earley \<G> \<omega> \<Longrightarrow> y = Item r\<^sub>y b\<^sub>y j k \<Longrightarrow> y \<in> Earley \<G> \<omega> \<Longrightarrow>
+  | Complete: "x = Item r\<^sub>x b\<^sub>x i j \<Longrightarrow> x \<in> Earley \<G> \<omega> \<Longrightarrow> y = Item r\<^sub>y b\<^sub>y j k \<Longrightarrow> y \<in> Earley \<G> \<omega> \<Longrightarrow>
     is_complete y \<Longrightarrow> next_symbol x = Some (item_rule_head y) \<Longrightarrow>
       Item r\<^sub>x (b\<^sub>x + 1) i k \<in> Earley \<G> \<omega>"
 
@@ -137,11 +132,11 @@ inductive_set Earley :: "'a cfg \<Rightarrow> 'a sentence \<Rightarrow> 'a item 
 subsection \<open>Well-formedness\<close>
 
 definition wf_item :: "'a cfg \<Rightarrow> 'a sentence => 'a item \<Rightarrow> bool" where 
-  "wf_item cfg inp x = (
-    item_rule x \<in> set (\<RR> cfg) \<and> 
+  "wf_item \<G> \<omega> x \<equiv>
+    item_rule x \<in> set (\<RR> \<G>) \<and> 
     item_dot x \<le> length (item_rule_body x) \<and>
     item_origin x \<le> item_end x \<and> 
-    item_end x \<le> length inp)"
+    item_end x \<le> length \<omega>"
 
 lemma wf_Init:
   assumes "r \<in> set (\<RR> \<G>)" "fst r = \<SS> \<G>"
@@ -175,7 +170,7 @@ lemma wf_Earley:
 subsection \<open>Soundness\<close>
 
 definition sound_item :: "'a cfg \<Rightarrow> 'a sentence \<Rightarrow> 'a item \<Rightarrow> bool" where
-  "sound_item \<G> \<omega> x = derives \<G> [item_rule_head x] (slice (item_origin x) (item_end x) \<omega> @ item_\<beta> x)"
+  "sound_item \<G> \<omega> x \<equiv> derives \<G> [item_rule_head x] (slice (item_origin x) (item_end x) \<omega> @ item_\<beta> x)"
 
 lemma sound_Init:
   assumes "r \<in> set (\<RR> \<G>)" "fst r = \<SS> \<G>"
@@ -266,12 +261,12 @@ next
     using wf_Earley sound_Complete by metis
 qed
 
-theorem soundness:
-  assumes "earley_recognized (Earley \<G> \<omega>) \<G> \<omega>"
+theorem soundness_Earley:
+  assumes "recognizing (Earley \<G> \<omega>) \<G> \<omega>"
   shows "derives \<G> [\<SS> \<G>] \<omega>"
 proof -
   obtain x where x: "x \<in> Earley \<G> \<omega>" "is_finished \<G> \<omega> x"
-    using assms earley_recognized_def by blast
+    using assms recognizing_def by blast
   hence "sound_item \<G> \<omega> x"
     using wf_Earley sound_Earley by blast
   thus ?thesis
@@ -282,13 +277,11 @@ qed
 subsection \<open>Completeness\<close>
 
 definition partially_completed :: "nat \<Rightarrow> 'a cfg \<Rightarrow> 'a sentence \<Rightarrow> 'a item set \<Rightarrow> ('a derivation \<Rightarrow> bool) \<Rightarrow> bool" where
-  "partially_completed k \<G> \<omega> E P = (
-    \<forall>r b i' i j x a D.
-      i \<le> j \<and> j \<le> k \<and> k \<le> length \<omega> \<and>
-      x = Item r b i' i \<and> x \<in> E \<and> next_symbol x = Some a \<and>
-      Derivation \<G> [a] D (slice i j \<omega>) \<and> P D \<longrightarrow>
-      Item r (b+1) i' j \<in> E
-  )"
+  "partially_completed k \<G> \<omega> E P \<equiv> \<forall>r b i' i j x a D.
+    i \<le> j \<and> j \<le> k \<and> k \<le> length \<omega> \<and>
+    x = Item r b i' i \<and> x \<in> E \<and> next_symbol x = Some a \<and>
+    Derivation \<G> [a] D (slice i j \<omega>) \<and> P D \<longrightarrow>
+    Item r (b+1) i' j \<in> E"
 
 lemma partially_completed_upto:
   assumes "j \<le> k" "k \<le> length \<omega>"
@@ -335,7 +328,7 @@ next
 qed
 
 lemma partially_completed_Earley_k:
-  assumes "wf_cfg \<G>"
+  assumes "wf_\<G> \<G>"
   shows "partially_completed k \<G> \<omega> (Earley \<G> \<omega>) (\<lambda>_. True)"
   unfolding partially_completed_def
 proof (standard, standard, standard, standard, standard, standard, standard, standard, standard)
@@ -372,7 +365,7 @@ proof (standard, standard, standard, standard, standard, standard, standard, sta
       then obtain \<alpha> where *: "Derives1 \<G> [a] (fst d) (snd d) \<alpha>" "Derivation \<G> \<alpha> D' (slice i j \<omega>)"
         using "1.prems" by auto
       hence rule: "(a, \<alpha>) \<in> set (\<RR> \<G>)" "fst d = 0" "snd d = (a ,\<alpha>)"
-          using *(1) unfolding Derives1_def by (simp add: Cons_eq_append_conv)+
+        using *(1) unfolding Derives1_def by (simp add: Cons_eq_append_conv)+
       show ?thesis
       proof cases
         assume "is_terminal \<G> a"
@@ -383,91 +376,38 @@ proof (standard, standard, standard, standard, standard, standard, standard, sta
       next
         assume "\<not> is_terminal \<G> a"
         define y where y_def: "y = Item (a ,\<alpha>) 0 i i"
-        have "y \<in> Earley \<G> \<omega>"
-          using y_def "1.prems" rule by (auto simp: item_defs Earley.Predict)
-        have "i \<le> j"
-          using "1.prems" by blast
-        have "j \<le> length \<omega>"
-          using "1.prems" by simp
         have "length D' < length D"
           using \<open>D = d # D'\<close> by fastforce
-
-        have "\<forall>m<length D.
-     \<forall>x. m = length x \<longrightarrow>
-         (\<forall>xa xb xc xd xe xf xg.
-             xd \<le> xe \<and> xe \<le> k \<and> k \<le> length \<omega> \<and> xf = Item xa xb xc xd \<and> xf \<in> Earley \<G> \<omega> \<and> next_symbol xf = Some xg
-              \<and> Derivation \<G> [xg] x (slice xd xe \<omega>) \<and> True \<longrightarrow>
-             Item xa (xb + 1) xc xe \<in> Earley \<G> \<omega>)"
-          using "1.hyps" by blast
-        hence "\<forall>m x.
-      m < length D \<and> m = length x \<longrightarrow>
-         (\<forall>xa xb xc xd xe xf xg.
-             xd \<le> xe \<and> xe \<le> k \<and> k \<le> length \<omega> \<and> xf = Item xa xb xc xd \<and> xf \<in> Earley \<G> \<omega> \<and> next_symbol xf = Some xg
-              \<and> Derivation \<G> [xg] x (slice xd xe \<omega>) \<and> True \<longrightarrow>
-             Item xa (xb + 1) xc xe \<in> Earley \<G> \<omega>)"
-          by blast
-        hence "\<forall>m x.
-      m \<le> length D' \<and> m = length x \<longrightarrow>
-         (\<forall>xa xb xc xd xe xf xg.
-             xd \<le> xe \<and> xe \<le> k \<and> k \<le> length \<omega> \<and> xf = Item xa xb xc xd \<and> xf \<in> Earley \<G> \<omega> \<and> next_symbol xf = Some xg
-              \<and> Derivation \<G> [xg] x (slice xd xe \<omega>) \<and> True \<longrightarrow>
-             Item xa (xb + 1) xc xe \<in> Earley \<G> \<omega>)"
-          by (smt (verit, best) \<open>length D' < length D\<close> order_le_less_trans)
-        hence "\<forall>x.
-         (\<forall>xa xb xc xd xe xf xg.
-             xd \<le> xe \<and> xe \<le> k \<and> k \<le> length \<omega> \<and> xf = Item xa xb xc xd \<and> xf \<in> Earley \<G> \<omega> \<and> next_symbol xf = Some xg
-              \<and> Derivation \<G> [xg] x (slice xd xe \<omega>) \<and> length x \<le> length D' \<longrightarrow>
-             Item xa (xb + 1) xc xe \<in> Earley \<G> \<omega>)"
-          by fast
         hence "partially_completed k \<G> \<omega> (Earley \<G> \<omega>) (\<lambda>E. length E \<le> length D')"
-          unfolding partially_completed_def by blast
-        hence 0: "partially_completed j \<G> \<omega> (Earley \<G> \<omega>) (\<lambda>E. length E \<le> length D')"
+          unfolding partially_completed_def using "1.hyps" order_le_less_trans by (smt (verit, best))
+        hence "partially_completed j \<G> \<omega> (Earley \<G> \<omega>) (\<lambda>E. length E \<le> length D')"
           unfolding partially_completed_def using "1.prems" by force
-
-        have 1: "Derivation \<G> (item_\<beta> y) D' (slice i j \<omega>)"
+        moreover have "Derivation \<G> (item_\<beta> y) D' (slice i j \<omega>)"
           using *(2) by (auto simp: item_defs y_def)
-        have 0: "Item (a,\<alpha>) (length \<alpha>) i j \<in> Earley \<G> \<omega>"
-          using partially_completed_upto by (metis "0" "1" "1.prems" \<open>j \<le> length \<omega>\<close> \<open>y \<in> Earley \<G> \<omega>\<close> wf_Earley y_def)
-
-        have 2: "x = Item r b i' i" "x \<in> Earley \<G> \<omega>"
+        moreover have "y \<in> Earley \<G> \<omega>"
+          using y_def "1.prems" rule by (auto simp: item_defs Earley.Predict)
+        moreover have "j \<le> length \<omega>"
+          using "1.prems" by simp
+        ultimately have "Item (a,\<alpha>) (length \<alpha>) i j \<in> Earley \<G> \<omega>"
+          using partially_completed_upto "1.prems" wf_Earley y_def by metis
+        moreover have x: "x = Item r b i' i" "x \<in> Earley \<G> \<omega>"
           using "1.prems" by blast+
-
-        have "j \<le> k"
-          using "1.prems" by blast
-        have "next_symbol x = Some a"
+        moreover have "next_symbol x = Some a"
           using "1.prems" by linarith
-        thus ?thesis
-          using Earley.Complete[OF 2 _ 0] by (auto simp: is_complete_def item_defs)
+        ultimately show ?thesis
+          using Earley.Complete[OF x] by (auto simp: is_complete_def item_defs)
       qed
     qed
   qed
 qed
 
 lemma partially_completed_Earley:
-  "wf_cfg \<G> \<Longrightarrow> partially_completed (length \<omega>) \<G> \<omega> (Earley \<G> \<omega>) (\<lambda>_. True)"
+  "wf_\<G> \<G> \<Longrightarrow> partially_completed (length \<omega>) \<G> \<omega> (Earley \<G> \<omega>) (\<lambda>_. True)"
   by (simp add: partially_completed_Earley_k)
 
-lemma Derivation_\<SS>1:
-  assumes "Derivation \<G> [\<SS> \<G>] D \<omega>" "is_word \<G> \<omega>" "wf_cfg \<G>"
-  shows "\<exists>\<alpha> E. Derivation \<G> \<alpha> E \<omega> \<and> (\<SS> \<G>,\<alpha>) \<in> set (\<RR> \<G>)"
-proof (cases D)
-  case Nil
-  thus ?thesis
-    using assms is_nonterminal_startsymbol is_terminal_nonterminal by (metis Derivation.simps(1) is_word_def list.set_intros(1))
-next
-  case (Cons d D)
-  then obtain \<alpha> where "Derives1 \<G> [\<SS> \<G>] (fst d) (snd d) \<alpha>" "Derivation \<G> \<alpha> D \<omega>"
-    using assms by auto
-  hence "(\<SS> \<G>, \<alpha>) \<in> set (\<RR> \<G>)"
-    unfolding Derives1_def
-    by (metis List.append.right_neutral List.list.discI append_eq_Cons_conv append_is_Nil_conv nth_Cons_0 self_append_conv2)
-  thus ?thesis
-    using \<open>Derivation \<G> \<alpha> D \<omega>\<close> by auto
-qed
-
-theorem completeness:
-  assumes "derives \<G> [\<SS> \<G>] \<omega>" "is_word \<G> \<omega>" "wf_cfg \<G>"
-  shows "earley_recognized (Earley \<G> \<omega>) \<G> \<omega>"
+theorem completeness_Earley:
+  assumes "derives \<G> [\<SS> \<G>] \<omega>" "is_word \<G> \<omega>" "wf_\<G> \<G>"
+  shows "recognizing (Earley \<G> \<omega>) \<G> \<omega>"
 proof -
   obtain \<alpha> D where *: "(\<SS> \<G> ,\<alpha>) \<in> set (\<RR> \<G>)" "Derivation \<G> \<alpha> D \<omega>"
     using Derivation_\<SS>1 assms derives_implies_Derivation by metis
@@ -483,49 +423,50 @@ proof -
   have "Item (\<SS> \<G>,\<alpha>) (length \<alpha>) 0 (length \<omega>) \<in> Earley \<G> \<omega>"
     using partially_completed_upto[OF _ _ _ _ _ 2 0] wf_Earley 1 x_def by auto
   then show ?thesis
-    unfolding earley_recognized_def is_finished_def by (auto simp: is_complete_def item_defs, force)
+    unfolding recognizing_def is_finished_def by (auto simp: is_complete_def item_defs, force)
 qed
+
 
 subsection \<open>Correctness\<close>
 
-corollary correctness:
-  assumes "wf_cfg cfg" "is_word cfg inp"
-  shows "earley_recognized (Earley cfg inp) cfg inp \<longleftrightarrow> derives cfg [\<SS> cfg] inp"
-  using assms soundness completeness by blast
+corollary correctness_Earley:
+  assumes "wf_\<G> \<G>" "is_word \<G> \<omega>"
+  shows "recognizing (Earley \<G> \<omega>) \<G> \<omega> \<longleftrightarrow> derives \<G> [\<SS> \<G>] \<omega>"
+  using assms soundness_Earley completeness_Earley by blast
 
 
 subsection \<open>Finiteness\<close>
 
 lemma finiteness_empty:
-  "set (\<RR> cfg) = {} \<Longrightarrow> finite { x | x. wf_item cfg inp x }"
+  "set (\<RR> \<G>) = {} \<Longrightarrow> finite { x | x. wf_item \<G> \<omega> x }"
   unfolding wf_item_def by simp
 
 fun item_intro :: "'a rule \<times> nat \<times> nat \<times> nat \<Rightarrow> 'a item" where
   "item_intro (rule, dot, origin, ends) = Item rule dot origin ends" 
 
 lemma finiteness_nonempty:
-  assumes "set (\<RR> cfg) \<noteq> {}"
-  shows "finite { x | x. wf_item cfg inp x }"
+  assumes "set (\<RR> \<G>) \<noteq> {}"
+  shows "finite { x | x. wf_item \<G> \<omega> x }"
 proof -
-  define M where "M = Max { length (rule_body r) | r. r \<in> set (\<RR> cfg) }"
-  define Top where "Top = (set (\<RR> cfg) \<times> {0..M} \<times> {0..length inp} \<times> {0..length inp})"
+  define M where "M = Max { length (rule_body r) | r. r \<in> set (\<RR> \<G>) }"
+  define Top where "Top = (set (\<RR> \<G>) \<times> {0..M} \<times> {0..length \<omega>} \<times> {0..length \<omega>})"
   hence "finite Top"
     using finite_cartesian_product finite by blast
   have "inj_on item_intro Top"
     unfolding Top_def inj_on_def by simp
   hence "finite (item_intro ` Top)"
     using finite_image_iff \<open>finite Top\<close> by auto
-  have "{ x | x. wf_item cfg inp x } \<subseteq> item_intro ` Top"
+  have "{ x | x. wf_item \<G> \<omega> x } \<subseteq> item_intro ` Top"
   proof standard
     fix x
-    assume "x \<in> { x | x. wf_item cfg inp x }"
+    assume "x \<in> { x | x. wf_item \<G> \<omega> x }"
     then obtain rule dot origin endp where *: "x = Item rule dot origin endp"
-      "rule \<in> set (\<RR> cfg)" "dot \<le> length (item_rule_body x)" "origin \<le> length inp" "endp \<le> length inp"
+      "rule \<in> set (\<RR> \<G>)" "dot \<le> length (item_rule_body x)" "origin \<le> length \<omega>" "endp \<le> length \<omega>"
       unfolding wf_item_def using item.exhaust_sel le_trans by blast
-    hence "length (rule_body rule) \<in> { length (rule_body r) | r. r \<in> set (\<RR> cfg) }"
+    hence "length (rule_body rule) \<in> { length (rule_body r) | r. r \<in> set (\<RR> \<G>) }"
       using *(1,2) item_rule_body_def by blast
-    moreover have "finite { length (rule_body r) | r. r \<in> set (\<RR> cfg) }"
-      using finite finite_image_set[of "\<lambda>x. x \<in> set (\<RR> cfg)"] by fastforce
+    moreover have "finite { length (rule_body r) | r. r \<in> set (\<RR> \<G>) }"
+      using finite finite_image_set[of "\<lambda>x. x \<in> set (\<RR> \<G>)"] by fastforce
     ultimately have "M \<ge> length (rule_body rule)"
       unfolding M_def by simp
     hence "dot \<le> M"
@@ -540,11 +481,11 @@ proof -
 qed
 
 lemma finiteness_UNIV_wf_item:
-  "finite { x | x. wf_item cfg inp x }"
+  "finite { x | x. wf_item \<G> \<omega> x }"
   using finiteness_empty finiteness_nonempty by fastforce
 
-theorem finiteness:
-  "finite (Earley cfg inp)"
+theorem finiteness_Earley:
+  "finite (Earley \<G> \<omega>)"
   using finiteness_UNIV_wf_item wf_Earley rev_finite_subset by (metis mem_Collect_eq subsetI)
 
 end
