Examples.thy
@@ -7,15 +7,15 @@ declare [[names_short]]
 section \<open>Epsilon Productions\<close>
 
 definition \<epsilon>_free :: "'a cfg \<Rightarrow> bool" where
-  "\<epsilon>_free cfg \<longleftrightarrow> (\<forall>r \<in> set (\<RR> cfg). rule_body r \<noteq> [])"
+  "\<epsilon>_free \<G> \<longleftrightarrow> (\<forall>r \<in> set (\<RR> \<G>). rule_body r \<noteq> [])"
 
 lemma \<epsilon>_free_impl_non_empty_sentence_deriv:
-  "\<epsilon>_free cfg \<Longrightarrow> a \<noteq> [] \<Longrightarrow> \<not> Derivation cfg a D []"
+  "\<epsilon>_free \<G> \<Longrightarrow> a \<noteq> [] \<Longrightarrow> \<not> Derivation \<G> a D []"
 proof (induction "length D" arbitrary: a D rule: nat_less_induct)
   case 1
   show ?case
   proof (rule ccontr)
-    assume assm: "\<not> \<not> Derivation cfg a D []"
+    assume assm: "\<not> \<not> Derivation \<G> a D []"
     show False
     proof (cases "D = []")
       case True
@@ -24,7 +24,7 @@ proof (induction "length D" arbitrary: a D rule: nat_less_induct)
     next
       case False
       then obtain d D' \<alpha> where *:
-        "D = d # D'" "Derives1 cfg a (fst d) (snd d) \<alpha>" "Derivation cfg \<alpha> D' []" "snd d \<in> set (\<RR> cfg)"
+        "D = d # D'" "Derives1 \<G> a (fst d) (snd d) \<alpha>" "Derivation \<G> \<alpha> D' []" "snd d \<in> set (\<RR> \<G>)"
         using list.exhaust assm Derives1_def by (metis Derivation.simps(2))
       show ?thesis
       proof cases
@@ -41,29 +41,29 @@ proof (induction "length D" arbitrary: a D rule: nat_less_induct)
 qed
 
 lemma \<epsilon>_free_impl_non_empty_deriv:
-  "\<epsilon>_free cfg \<Longrightarrow> \<forall>N \<in> set (\<NN> cfg). \<not> derives cfg [N] []"
+  "\<epsilon>_free \<G> \<Longrightarrow> \<forall>N \<in> set (\<NN> \<G>). \<not> derives \<G> [N] []"
   using \<epsilon>_free_impl_non_empty_sentence_deriv derives_implies_Derivation by (metis not_Cons_self2)
 
 lemma nonempty_deriv_impl_\<epsilon>_free:
-  assumes "\<forall>N \<in> set (\<NN> cfg). \<not> derives cfg [N] []" "\<forall>(N, \<alpha>) \<in> set (\<RR> cfg). N \<in> set (\<NN> cfg)"
-  shows "\<epsilon>_free cfg"
+  assumes "\<forall>N \<in> set (\<NN> \<G>). \<not> derives \<G> [N] []" "\<forall>(N, \<alpha>) \<in> set (\<RR> \<G>). N \<in> set (\<NN> \<G>)"
+  shows "\<epsilon>_free \<G>"
 proof (rule ccontr)
-  assume "\<not> \<epsilon>_free cfg"
-  then obtain N \<alpha> where *: "(N, \<alpha>) \<in> set (\<RR> cfg)" "rule_body (N, \<alpha>) = []"
+  assume "\<not> \<epsilon>_free \<G>"
+  then obtain N \<alpha> where *: "(N, \<alpha>) \<in> set (\<RR> \<G>)" "rule_body (N, \<alpha>) = []"
     unfolding \<epsilon>_free_def by auto
-  hence "derives1 cfg [N] []"
+  hence "derives1 \<G> [N] []"
     unfolding derives1_def rule_body_def by auto
-  hence "derives cfg [N] []"
+  hence "derives \<G> [N] []"
     by auto
-  moreover have "N \<in> set (\<NN> cfg)"
+  moreover have "N \<in> set (\<NN> \<G>)"
     using *(1) assms(2) by blast
   ultimately show False
     using assms(1) by blast
 qed
 
 lemma nonempty_deriv_iff_\<epsilon>_free:
-  assumes "\<forall>(N, \<alpha>) \<in> set (\<RR> cfg). N \<in> set (\<NN> cfg)"
-  shows "(\<forall>N \<in> set (\<NN> cfg). \<not> derives cfg [N] []) \<longleftrightarrow> \<epsilon>_free cfg"
+  assumes "\<forall>(N, \<alpha>) \<in> set (\<RR> \<G>). N \<in> set (\<NN> \<G>)"
+  shows "(\<forall>N \<in> set (\<NN> \<G>). \<not> derives \<G> [N] []) \<longleftrightarrow> \<epsilon>_free \<G>"
   using \<epsilon>_free_impl_non_empty_deriv nonempty_deriv_impl_\<epsilon>_free[OF _ assms] by blast
 
 section \<open>Example 1: Addition\<close>
@@ -95,9 +95,9 @@ definition inp1 :: "s1 list" where
 
 lemmas cfg1_defs = cfg1_def nonterminals1_def terminals1_def rules1_def start_symbol1_def
 
-lemma wf_cfg1:
-  "wf_cfg cfg1"
-  by (auto simp: wf_cfg_defs cfg1_defs)
+lemma wf_\<G>1:
+  "wf_\<G> cfg1"
+  by (auto simp: wf_\<G>_defs cfg1_defs)
 
 lemma is_word_inp1:
   "is_word cfg1 inp1"
@@ -109,26 +109,26 @@ lemma nonempty_derives1:
 
 lemma correctness1:
   "earley_recognized_it (\<II>_it cfg1 inp1) cfg1 inp1 \<longleftrightarrow> derives cfg1 [\<SS> cfg1] inp1"
-  using correctness_list wf_cfg1 is_word_inp1 nonempty_derives1 by blast
+  using correctness_list wf_\<G>1 is_word_inp1 nonempty_derives1 by blast
 
 lemma wf_tree1:
   assumes "build_tree cfg1 inp1 (\<II>_it cfg1 inp1) = Some t"
   shows "wf_rule_tree cfg1 t \<and> root_tree t = \<SS> cfg1 \<and> yield_tree t = inp1"
-  using assms nonempty_derives1 wf_cfg1 wf_rule_root_yield_tree_build_tree_\<II>_it by blast
+  using assms nonempty_derives1 wf_\<G>1 wf_rule_root_yield_tree_build_tree_\<II>_it by blast
 
 lemma correctness_tree1:
   "(\<exists>t. build_tree cfg1 inp1 (\<II>_it cfg1 inp1) = Some t) \<longleftrightarrow> derives cfg1 [\<SS> cfg1] inp1"
-  using correctness_build_tree_\<II>_it is_word_inp1 nonempty_derives1 wf_cfg1 by blast
+  using correctness_build_tree_\<II>_it is_word_inp1 nonempty_derives1 wf_\<G>1 by blast
 
 lemma wf_trees1:
   assumes "build_trees cfg1 inp1 (\<II>_it cfg1 inp1) = Some fs" "f \<in> set fs" "t \<in> set (trees f)"
   shows "wf_rule_tree cfg1 t \<and> root_tree t = \<SS> cfg1 \<and> yield_tree t = inp1"
-  using assms nonempty_derives1 wf_cfg1 wf_rule_root_yield_tree_build_trees_\<II>_it by blast
+  using assms nonempty_derives1 wf_\<G>1 wf_rule_root_yield_tree_build_trees_\<II>_it by blast
 
 lemma soundness_trees1:
   assumes "build_trees cfg1 inp1 (\<II>_it cfg1 inp1) = Some fs" "f \<in> set fs" "t \<in> set (trees f)"
   shows "derives cfg1 [\<SS> cfg1] inp1"
-  using assms is_word_inp1 nonempty_derives1 soundness_build_trees_\<II>_it wf_cfg1 by blast
+  using assms is_word_inp1 nonempty_derives1 soundness_build_trees_\<II>_it wf_\<G>1 by blast
 
 section \<open>Example 2: Cyclic reduction pointers\<close>
 
@@ -160,9 +160,9 @@ definition inp2 :: "s2 list" where
 
 lemmas cfg2_defs = cfg2_def nonterminals2_def terminals2_def rules2_def start_symbol2_def
 
-lemma wf_cfg2:
-  "wf_cfg cfg2"
-  by (auto simp: wf_cfg_defs cfg2_defs)
+lemma wf_\<G>2:
+  "wf_\<G> cfg2"
+  by (auto simp: wf_\<G>_defs cfg2_defs)
 
 lemma is_word_inp2:
   "is_word cfg2 inp2"
@@ -174,26 +174,26 @@ lemma nonempty_derives2:
 
 lemma correctness2:
   "earley_recognized_it (\<II>_it cfg2 inp2) cfg2 inp2 \<longleftrightarrow> derives cfg2 [\<SS> cfg2] inp2"
-  using correctness_list wf_cfg2 is_word_inp2 nonempty_derives2 by blast
+  using correctness_list wf_\<G>2 is_word_inp2 nonempty_derives2 by blast
 
 lemma wf_tree2:
   assumes "build_tree cfg2 inp2 (\<II>_it cfg2 inp2) = Some t"
   shows "wf_rule_tree cfg2 t \<and> root_tree t = \<SS> cfg2 \<and> yield_tree t = inp2"
-  using assms nonempty_derives2 wf_cfg2 wf_rule_root_yield_tree_build_tree_\<II>_it by blast
+  using assms nonempty_derives2 wf_\<G>2 wf_rule_root_yield_tree_build_tree_\<II>_it by blast
 
 lemma correctness_tree2:
   "(\<exists>t. build_tree cfg2 inp2 (\<II>_it cfg2 inp2) = Some t) \<longleftrightarrow> derives cfg2 [\<SS> cfg2] inp2"
-  using correctness_build_tree_\<II>_it is_word_inp2 nonempty_derives2 wf_cfg2 by blast
+  using correctness_build_tree_\<II>_it is_word_inp2 nonempty_derives2 wf_\<G>2 by blast
 
 lemma wf_trees2:
   assumes "build_trees cfg2 inp2 (\<II>_it cfg2 inp2) = Some fs" "f \<in> set fs" "t \<in> set (trees f)"
   shows "wf_rule_tree cfg2 t \<and> root_tree t = \<SS> cfg2 \<and> yield_tree t = inp2"
-  using assms nonempty_derives2 wf_cfg2 wf_rule_root_yield_tree_build_trees_\<II>_it by blast
+  using assms nonempty_derives2 wf_\<G>2 wf_rule_root_yield_tree_build_trees_\<II>_it by blast
 
 lemma soundness_trees2:
   assumes "build_trees cfg2 inp2 (\<II>_it cfg2 inp2) = Some fs" "f \<in> set fs" "t \<in> set (trees f)"
   shows "derives cfg2 [\<SS> cfg2] inp2"
-  using assms is_word_inp2 nonempty_derives2 soundness_build_trees_\<II>_it wf_cfg2 by blast
+  using assms is_word_inp2 nonempty_derives2 soundness_build_trees_\<II>_it wf_\<G>2 by blast
 
 unused_thms CFG -
 
